KripkeGameAnalysis/Generic/HashSetModExt.lean
@@ -1,0 +1,110 @@
+import KripkeGameAnalysis.GenericExtras.HashSet
+import Mathlib.Data.Quot
+import Mathlib.Data.Finset.Basic
+import Mathlib.Data.Multiset.MapFold
+import Batteries.Data.List.Perm
+
+def HashSetExtensionality {α : Type} [BEq α] [Hashable α] [Hashable α] : Setoid (Std.HashSet α) where
+  r := fun s t => ∀ x, (x ∈ s) = (x ∈ t)
+  iseqv := {
+    refl := by intros; trivial
+    symm := by
+      intro s t h x
+      exact (h x).symm
+    trans := by
+      intro s t u hst htu x
+      rw [hst x]
+      exact htu x
+  }
+
+abbrev HashSetModExt (α : Type) [BEq α] [Hashable α] : Type := Quotient (HashSetExtensionality (α := α))
+namespace HashSetModExt
+
+section
+variable {α : Type} [BEq α] [Hashable α]
+
+def empty : HashSetModExt α := ⟦∅⟧
+instance : EmptyCollection (HashSetModExt α) := ⟨empty⟩
+
+theorem emptyc_toList_eq_nil [EquivBEq α] [LawfulHashable α]: (∅ : Std.HashSet α).toList = [] := by
+  apply List.eq_nil_of_length_eq_zero
+  rw [Std.HashSet.length_toList]
+  exact Std.HashSet.size_emptyc
+
+end
+
+section
+variable {α : Type} [BEq α] [Hashable α] [EquivBEq α] [LawfulHashable α] [LawfulBEq α]
+
+def toFinset (s : HashSetModExt α) : Finset α :=
+  s.liftOn (fun s => {
+    val := s.toList,
+    nodup := Std.HashSet.distinct_toList_nodup s
+  }) (by
+    intro s t s_ext_t
+    suffices _ : s.toList.Perm t.toList by simpa
+    rw [List.perm_ext_iff_of_nodup (Std.HashSet.distinct_toList_nodup s) (Std.HashSet.distinct_toList_nodup t)]
+    intro a
+    simp only [Std.HashSet.mem_toList, s_ext_t a]
+  )
+
+end
+
+section
+variable {α : Type} [BEq α] [Hashable α]
+
+def contains (s : HashSetModExt α) (a : α) : Bool :=
+  s.liftOn (a ∈ ·) (by intro _ _ e; simp [e a])
+
+instance : Membership α (HashSetModExt α) where
+  mem s a := contains s a
+
+@[simp] theorem contains_iff_mem {s : Std.HashSet α}
+                                 {a : α} : (a ∈ (⟦s⟧ : HashSetModExt α)) = (a ∈ s) := by
+  simp only [instMembership, contains, Quotient.lift_mk, decide_eq_true_eq]
+
+@[ext] theorem ext (s t : HashSetModExt α) (h : ∀ a, a ∈ s ↔ a ∈ t) : s = t := by
+  revert h
+  apply s.ind; apply t.ind
+  intro s_repr t_repr h
+  apply Quot.sound
+  intro a
+  rw [←contains_iff_mem, ←contains_iff_mem, h]
+
+end
+
+section
+variable {α : Type} [BEq α] [Hashable α] [EquivBEq α] [LawfulHashable α] [LawfulBEq α]
+
+def insert (s : HashSetModExt α) (a : α) : HashSetModExt α :=
+  s.liftOn (fun s => ⟦s.insert a⟧) (by
+    intro s t s_ext_t
+    apply Quot.sound; intro x
+    simp only [Std.HashSet.mem_insert, s_ext_t x]
+  )
+
+@[simp] theorem mem_insert { m: HashSetModExt α } { k a : α } : (a ∈ insert m k) ↔ (a == k ∨ a ∈ m) := by
+  apply m.ind; intro hs
+  suffices _ : k = a ∨ a ∈ hs ↔ a = k ∨ a ∈ hs by simpa [insert]
+  tauto
+
+instance insert_instRightCommutative: (RightCommutative (insert : HashSetModExt α -> α -> HashSetModExt α)) := by
+  apply RightCommutative.mk; intro s a b; ext x
+  simp only [mem_insert, beq_iff_eq]
+  tauto
+
+def insertAllOfFinset (s : HashSetModExt α) (fs : Finset α) : HashSetModExt α :=
+  fs.val.foldl insert s
+
+theorem mem_insertAllOfFinset { m: HashSetModExt α } { fs : Finset α }
+                              { a : α } : (a ∈ insertAllOfFinset m fs) ↔ (a ∈ fs ∨ a ∈ m) := by
+  dsimp only [insertAllOfFinset, Finset.instMembership]
+  induction fs.val using Multiset.induction generalizing m
+  next => simp
+  next fs_head fs ih =>
+    clear * - ih
+    simp only [Multiset.foldl_cons, ih, mem_insert, beq_iff_eq, Multiset.mem_cons]
+    tauto
+end
+
+end HashSetModExt
