KripkeGameAnalysis/GenericExtras/HashSet.lean
@@ -1,0 +1,16 @@
+import Std.Data.HashSet
+import Mathlib.Data.Multiset.Defs
+
+variable {a : Type} [BEq a] [Hashable a] [EquivBEq a] [LawfulHashable a]
+
+theorem Std.HashSet.emptyc_toList_eq_nil : (∅ : Std.HashSet a).toList = [] := by
+  apply List.eq_nil_of_length_eq_zero
+  rw [Std.HashSet.length_toList]
+  exact Std.HashSet.size_emptyc
+
+theorem Std.HashSet.distinct_toList_nodup [LawfulBEq a] (s : Std.HashSet a) : s.toList.Nodup := by
+  apply Multiset.coe_nodup.mpr
+  unfold List.Nodup
+  refine (List.Pairwise.imp ?_ Std.HashSet.distinct_toList)
+  intro a b
+  simp
